map
git-svn-id: svn://scm.gforge.inria.fr/svn/cfml@191 ba02c806-7d2b-4818-9a48-35b22e6bdc79

imper/MutableList_proof.v
@@ -1,9 +1,196 @@
 Set Implicit Arguments.
-Require Import LibCore CFPrim ListRev_ml LibList.
+Require Import LibCore CFPrim MutableList_ml LibList.
 
 Opaque List Ref.
 
-(*****************)
+
+
+(*------------------------------------------------------------------*)
+(* ** MListsSeg *)
+(*--todo: define MList as MListSeg null *)
+
+Fixpoint MListSeg (e:loc) A a (T:A->a->hprop) (L:list A) (l:loc) : hprop :=
+  match L with
+  | nil => [l = e]
+  | X::L' => l ~> Ref2 T (MListSeg e T) X L'
+  end.
+
+Lemma focus_msnil : forall (e:loc) A a (T:A->a->hprop),
+  [] ==> e ~> MListSeg e T nil.
+Proof. intros. simpl. hdata_simpl. hsimpl~. Qed.
+
+Lemma unfocus_msnil : forall (l e:loc) A a (T:A->a->hprop),
+  l ~> MListSeg e T nil ==> [l = e].
+Proof. intros. simpl. hdata_simpl. hsimpl~. Qed.
+
+Lemma unfocus_msnil' : forall A (L:list A) (e:loc) a (T:A->a->hprop),
+  null ~> MListSeg e T L ==> [L = nil] \* [e = null].
+Proof.
+  intros. destruct L.
+  simpl. unfold hdata. xsimpl~. 
+  unfold hdata, MListSeg. hchange focus_ref2_null. hextract. false.
+Qed.
+
+Lemma focus_mscons : forall (l e:loc) a A (X:A) (L':list A) (T:A->a->hprop),
+  (l ~> MListSeg e T (X::L')) ==>
+  Hexists x l', (x ~> T X) \* (l' ~> MListSeg e T L') \* (l ~> Ref Id (x,l')).
+Proof.
+  intros. simpl. hdata_simpl. hchange (@focus_ref2 l). xsimpl.
+Qed.
+
+Lemma focus_mscons' : forall (l e:loc) a A (L:list A) (T:A->a->hprop),
+  [l <> e] \* (l ~> MListSeg e T L) ==> 
+  Hexists x l', Hexists X L', 
+    [L = X::L'] \*  (l ~> Ref Id (x,l')) \* (x ~> T X) \* (l' ~> MListSeg e T L').
+Proof.
+  intros. destruct L. lets: (@unfocus_msnil l e _ _ T). (* Show Existentials. *)
+  hextract. false~.
+  hchange (@focus_mscons l e). hextract as x l' E. hsimpl~.  
+Qed.
+
+Lemma unfocus_mscons : forall (l:loc) a (x:a) (l' e:loc) A (X:A) (L':list A) (T:A->a->hprop),
+  (l ~> Ref Id (x,l')) \* (x ~> T X) \* (l' ~> MListSeg e T L') ==> 
+  (l ~> MListSeg e T (X::L')).
+Proof.
+  intros. simpl. hdata_simpl. hchange (@unfocus_ref2 l _ x _ l'). hsimpl.
+Qed.
+
+Opaque MListSeg.
+
+
+
+(********************************************************************)
+(* ** Accessors *)
+
+Lemma unfocus_mnil'' : forall (l:loc) A (L:list A) a (T:A->a->hprop),
+  l ~> MList T L ==> [l = null <-> L = nil] \* l ~> MList T L.
+Proof. skip. (*todo*) Qed.
+
+(*
+Implicit Arguments focus_mnil.
+Implicit Arguments unfocus_mnil.
+Implicit Arguments unfocus_mnil'.
+Implicit Arguments focus_mcons.
+Implicit Arguments focus_mcons'.
+Implicit Arguments unfocus_mcons.
+*)
+
+Lemma is_nil_spec : forall a,
+  Spec is_nil (l:mlist a) |R>> forall A (T:A->a->hprop) (L:list A),
+     keep R (l ~> MList T L) (\[ bool_of (L = nil) ]).
+Proof.
+  xcf. intros. xapp. intros b. hextract.
+  hchange (unfocus_mnil'' l). hextract. subst b. hsimpl. xclean. iff*.
+Qed.
+
+Module ML := MutableList_ml.
+
+Tactic Notation "xapps" :=
+  xapp; try intro_subst.
+
+Lemma head_spec : forall a,
+  Spec ML.head (l:mlist a) |R>> forall (x:a) (t:mlist a),
+    keep R (l ~> Ref Id (x,t)) (\= x).
+Proof. 
+  xcf. intros. xapps. xret.
+Qed.
+
+Lemma tail_spec : forall a,
+  Spec ML.tail (l:mlist a) |R>> forall (x:a) (t:mlist a),
+    keep R (l ~> Ref Id (x,t)) (\= t).
+Proof. 
+  xcf. intros. xapps. xret.
+Qed.
+
+Lemma set_head_spec : forall a,
+  Spec ML.set_head (x:a) (l:mlist a) |R>> forall (x':a) (t:mlist a),
+    R (l ~> Ref Id (x',t)) (# l ~> Ref Id (x,t)).
+Proof. 
+  xcf. intros. xapps. xmatch. xapp. hsimpl.
+Qed.
+
+Lemma set_tail_spec : forall a,
+  Spec ML.set_tail (t:mlist a) (l:mlist a) |R>> forall (x:a) (t':mlist a),
+    R (l ~> Ref Id (x,t)) (# l ~> Ref Id (x,t)).
+Proof. 
+  xcf. intros. xapps. xmatch. xapp. hsimpl.
+Qed.
+
+
+Hint Extern 1 (RegisterSpec is_nil) => Provide is_nil_spec.
+Hint Extern 1 (RegisterSpec ML.head) => Provide head_spec.
+Hint Extern 1 (RegisterSpec ML.tail) => Provide tail_spec.
+Hint Extern 1 (RegisterSpec ML.set_head) => Provide set_head_spec.
+Hint Extern 1 (RegisterSpec ML.set_tail) => Provide set_tail_spec.
+
+
+
+
+
+(********************************************************************)
+(* ** Destructive append *)
+
+Implicit Arguments unfocus_msnil [ ].
+Implicit Arguments focus_mscons [ ].
+Implicit Arguments unfocus_mscons [ a A ].
+
+Lemma focus_msapp : forall (l l' e:loc) a A (L L':list A) (T:A->a->hprop),
+  l ~> MListSeg l' T L \* l' ~> MListSeg e T L' ==> l ~> MListSeg e T (L++L').
+Proof.
+  intros l l' e a A L L' T. gen l. induction L as [|X R]; intros.
+  hchange (unfocus_msnil l). hextract. subst. auto.
+  rew_app. hchange (focus_mscons l). hextract as x r. hchange (IHR r).
+   hchange (unfocus_mscons l x r e X (R++L')). hsimpl.
+Qed.
+
+Axiom mlistseg_to_mlist : forall (l:loc) a A (T:htype A a) L,
+   l ~> MListSeg null T L ==> l ~> MList T L.
+Axiom mlist_to_mlistseg : forall (l:loc) a A (T:htype A a) L,
+   l ~> MList T L ==> l ~> MListSeg null T L.
+
+Lemma mappend_spec : forall a,
+  Spec mappend (l1:mlist a) (l2:mlist a) |R>> forall A (T:A->a->hprop) (L1 L2:list A),
+     R (l1 ~> MList T L1 \* l2 ~> MList T L2) (\= (length L : int)).
+Proof.
+  xcf. unfold mlist. intros.
+  xapp. xapp. xseq (Hexists l', n ~> @RefOn int (length L) \* p ~> RefOn l' \* l' ~> List T nil).
+    (* todo : xseq automatic if xwhile *)
+  xuntag. apply local_erase. exists (list A) (fun L' => Hexists k:int, Hexists l',
+     n ~> RefOn k \* p ~> RefOn l' \* l' ~> List T L' \* [k + length L' = length L]) (@list_sub A).
+  splits. prove_wf. exists L. hsimpl. math.
+  intros L'. xextract. intros k l' E. apply local_erase. 
+  skip.
+  intros l'. xgc. xapp. xsimpl. auto. 
+Qed.
+
+
+
+
+(********************************************************************)
+(* ** Length *)
+(*
+Lemma mlength_spec : forall a,
+  Spec mlength (l:mlist a) |R>> forall A (T:A->a->hprop) (L:list A),
+     R (l ~> List T L) (\= (length L : int)).
+Proof.
+  xcf. unfold mlist. intros.
+  xapp. xapp. xseq (Hexists l', n ~> @RefOn int (length L) \* p ~> RefOn l' \* l' ~> List T nil).
+    (* todo : xseq automatic if xwhile *)
+  xuntag. apply local_erase. exists (list A) (fun L' => Hexists k:int, Hexists l',
+     n ~> RefOn k \* p ~> RefOn l' \* l' ~> List T L' \* [k + length L' = length L]) (@list_sub A).
+  splits. prove_wf. exists L. hsimpl. math.
+  intros L'. xextract. intros k l' E. apply local_erase. 
+  skip.
+  intros l'. xgc. xapp. xsimpl. auto. 
+Qed.
+*)
+
+
+(********************************************************************)
+(* ** In place reversal *)
+
+
+(*-------------
 
 Lemma rev_spec : forall a,
   Spec ListRev_ml.rev (l:mlist a) |R>> forall A (T:A->a->hprop) (L:list A),
@@ -44,23 +231,6 @@ Qed.
 
 
 
-(*****************)
-(*
-Lemma mlength_spec : forall a,
-  Spec mlength (l:mlist a) |R>> forall A (T:A->a->hprop) (L:list A),
-     R (l ~> List T L) (\= (length L : int)).
-Proof.
-  xcf. unfold mlist. intros.
-  xapp. xapp. xseq (Hexists l', n ~> @RefOn int (length L) \* p ~> RefOn l' \* l' ~> List T nil).
-    (* todo : xseq automatic if xwhile *)
-  xuntag. apply local_erase. exists (list A) (fun L' => Hexists k:int, Hexists l',
-     n ~> RefOn k \* p ~> RefOn l' \* l' ~> List T L' \* [k + length L' = length L]) (@list_sub A).
-  splits. prove_wf. exists L. hsimpl. math.
-  intros L'. xextract. intros k l' E. apply local_erase. 
-  skip.
-  intros l'. xgc. xapp. xsimpl. auto. 
-Qed.
-*)
 
 
   (*
@@ -74,6 +244,7 @@ Qed.
 
 
 
+-------------*)
 
 
 
